\begin{enumerate}
	\item[a)]
		\begin{equation*}
			\begin{split}
				Var[Y] 	&= \frac{(2n - (-2n))(2n-(-2n)+2)}{12}\\
						&= \frac{(4n)(4n + 2)}{12}\\
						&= \frac{16n^2 + 8n}{12}\\
						&= \frac{4n^2+2}{3}\\
			\end{split}
		\end{equation*}
	\item[b)] 
		\begin{equation*}
			\begin{split}
				P(||Y-0|\ge n) 	&\leq \frac{Var[Y]}{n^2}\\
								&\leq \frac{\frac{4n^2+2}{3}}{n^2}\\
								&\leq \frac{4n^2+2}{3 n^2}\\
			\end{split}
		\end{equation*}
		Untersucht man nun den Grenzwert zeigt sich
		\begin{equation*}
			\begin{split}
				\lim\limits_{n \rightarrow \infty} \frac{4n^2+2}{3n^2} = \lim\limits_{n \rightarrow \infty} \frac{n^2(4+\frac{2}{n^2})}{n^2(3)} = \frac{4}{3}
			\end{split}
		\end{equation*}
		Die Absch√§tzung ist somit trivial.
\end{enumerate}